Restore atomicreduce (with admits), also fix bug in atomics.h

dist/Kuiper_AtomicReduce.cu
@@ -2,35 +2,79 @@
 
 #include "Kuiper_AtomicReduce.h"
 
+__global__
+
+static void __hoisted_0(uint32_t *a, uint32_t *gr)
+{
+  atomic_add_u32(gr, a[blockIdx_x()]);
+}
+
 uint32_t Kuiper_AtomicReduce_reduce_u32(size_t n, uint32_t *a)
 {
-  KRML_MAYBE_UNUSED_VAR(n);
-  KRML_MAYBE_UNUSED_VAR(a);
-  KRML_HOST_EPRINTF("KaRaMeL abort at %s:%d\n%s\n", __FILE__, __LINE__, "");
-  KRML_HOST_EXIT(255U);
+  uint32_t r = 0U;
+  uint32_t *gr = (uint32_t *)KPR_GPU_ALLOC((size_t)4U);
+  MUST(cudaMemcpy(gr, &r, (size_t)4U, cudaMemcpyHostToDevice));
+  KPR_KCALL(__hoisted_0, n, (size_t)1U, (size_t)1U, (size_t)0U, a, gr);
+  cudaDeviceSynchronize();
+  MUST(cudaMemcpy(&r, gr, (size_t)4U, cudaMemcpyDeviceToHost));
+  MUST(cudaFree(gr));
+  return r;
+}
+
+__global__
+
+static void __hoisted_1(uint64_t *a, uint64_t *gr)
+{
+  atomic_add_u64(gr, a[blockIdx_x()]);
 }
 
 uint64_t Kuiper_AtomicReduce_reduce_u64(size_t n, uint64_t *a)
 {
-  KRML_MAYBE_UNUSED_VAR(n);
-  KRML_MAYBE_UNUSED_VAR(a);
-  KRML_HOST_EPRINTF("KaRaMeL abort at %s:%d\n%s\n", __FILE__, __LINE__, "");
-  KRML_HOST_EXIT(255U);
+  uint64_t r = 0ULL;
+  uint64_t *gr = (uint64_t *)KPR_GPU_ALLOC((size_t)8U);
+  MUST(cudaMemcpy(gr, &r, (size_t)8U, cudaMemcpyHostToDevice));
+  KPR_KCALL(__hoisted_1, n, (size_t)1U, (size_t)1U, (size_t)0U, a, gr);
+  cudaDeviceSynchronize();
+  MUST(cudaMemcpy(&r, gr, (size_t)8U, cudaMemcpyDeviceToHost));
+  MUST(cudaFree(gr));
+  return r;
+}
+
+__global__
+
+static void __hoisted_2(float_t *a, float_t *gr)
+{
+  atomic_add_f32(gr, a[blockIdx_x()]);
 }
 
 float_t Kuiper_AtomicReduce_reduce_f32(size_t n, float_t *a)
 {
-  KRML_MAYBE_UNUSED_VAR(n);
-  KRML_MAYBE_UNUSED_VAR(a);
-  KRML_HOST_EPRINTF("KaRaMeL abort at %s:%d\n%s\n", __FILE__, __LINE__, "");
-  KRML_HOST_EXIT(255U);
+  float_t r = (float_t)0.0f;
+  float_t *gr = (float_t *)KPR_GPU_ALLOC((size_t)4U);
+  MUST(cudaMemcpy(gr, &r, (size_t)4U, cudaMemcpyHostToDevice));
+  KPR_KCALL(__hoisted_2, n, (size_t)1U, (size_t)1U, (size_t)0U, a, gr);
+  cudaDeviceSynchronize();
+  MUST(cudaMemcpy(&r, gr, (size_t)4U, cudaMemcpyDeviceToHost));
+  MUST(cudaFree(gr));
+  return r;
+}
+
+__global__
+
+static void __hoisted_3(double_t *a, double_t *gr)
+{
+  atomic_add_f64(gr, a[blockIdx_x()]);
 }
 
 double_t Kuiper_AtomicReduce_reduce_f64(size_t n, double_t *a)
 {
-  KRML_MAYBE_UNUSED_VAR(n);
-  KRML_MAYBE_UNUSED_VAR(a);
-  KRML_HOST_EPRINTF("KaRaMeL abort at %s:%d\n%s\n", __FILE__, __LINE__, "");
-  KRML_HOST_EXIT(255U);
+  double_t r = (double_t)0.0l;
+  double_t *gr = (double_t *)KPR_GPU_ALLOC((size_t)8U);
+  MUST(cudaMemcpy(gr, &r, (size_t)8U, cudaMemcpyHostToDevice));
+  KPR_KCALL(__hoisted_3, n, (size_t)1U, (size_t)1U, (size_t)0U, a, gr);
+  cudaDeviceSynchronize();
+  MUST(cudaMemcpy(&r, gr, (size_t)8U, cudaMemcpyDeviceToHost));
+  MUST(cudaFree(gr));
+  return r;
 }
 
